Valaig/Aig/NodeArray.lean
@@ -1,0 +1,165 @@
+module
+
+public import Valaig.Refs
+
+public section
+namespace Valaig.Aig
+
+/--
+  The internal datastructure used to define an array of nodes in the Aig.
+  This is an implementation detail and should not be relied upon.
+-/
+structure NodeArray where
+  _nodes : Array Lit
+  _size : Nat
+  nonempty : _size > 0 := by grind
+  pairs : _nodes.size = 2 * _size := by grind
+deriving Repr, DecidableEq
+
+namespace NodeArray
+variable {var : Var} {arr : NodeArray}
+
+attribute [local grind =] NodeArray.pairs
+attribute [local grind! .] NodeArray.nonempty
+
+@[grind .]
+theorem two_dvd_nodes_size :
+    2 ∣ arr._nodes.size := by
+  grind
+
+@[always_inline, local simp, local grind]
+def size (arr : NodeArray) : Nat :=
+  arr._size
+
+@[simp, grind! .]
+theorem zero_lt_size :
+    0 < arr.size := by
+  grind
+
+instance : Membership Var NodeArray where
+  mem arr var := var.idx < arr.size
+
+@[simp, grind =]
+theorem mem_iff :
+    var ∈ arr ↔ var.idx < arr.size := by
+  rfl
+
+@[always_inline]
+instance : Decidable (var ∈ arr) :=
+  decidable_of_iff' _ mem_iff
+
+structure Elem where
+  arr : NodeArray
+  idx : Nat
+  valid : idx < arr._nodes.size := by grind
+  dvd : 2 ∣ idx := by grind
+
+attribute [local grind .] Elem.dvd
+attribute [local grind! .] Elem.valid
+
+@[always_inline]
+instance instGetElem : GetElem NodeArray Var Elem Membership.mem where
+  getElem arr var h := .mk arr (2 * var.idx)
+
+@[simp, grind =]
+private theorem arr_getElem (mem : var ∈ arr) :
+  (arr[var]'mem).arr = arr := by
+  simp +instances [GetElem.getElem]
+
+namespace Elem
+variable {elem : Elem}
+
+@[always_inline]
+def fst (elem : Elem) : Lit :=
+  elem.arr._nodes[elem.idx]
+
+@[always_inline]
+def snd (elem : Elem) : Lit :=
+  elem.arr._nodes[elem.idx + 1]
+
+@[coe, always_inline]
+def toPair (elem : Elem) : (Lit × Lit) :=
+  (elem.fst, elem.snd)
+
+@[always_inline]
+instance : Coe Elem (Lit × Lit) where
+  coe := Elem.toPair
+
+@[simp, grind =]
+theorem fst_eq :
+    elem.fst = elem.toPair.fst := by
+  grind [toPair]
+
+@[simp, grind =]
+theorem snd_eq :
+    elem.snd = elem.toPair.snd := by
+  grind [toPair]
+
+end Elem
+
+attribute [local grind] Elem.toPair Elem.fst Elem.snd
+
+@[local simp, local grind =]
+private theorem fst_toPair_getElem (mem : var ∈ arr) :
+    (arr[var]'mem).toPair.fst = arr._nodes[2 * var.idx] := by
+  simp only [Elem.toPair, Elem.fst, instGetElem]
+
+@[local simp, local grind =]
+private theorem snd_toPair_getElem (mem : var ∈ arr) :
+    (arr[var]'mem).toPair.snd = arr._nodes[2 * var.idx + 1] := by
+  simp only [Elem.toPair, Elem.snd, instGetElem]
+
+@[always_inline]
+def empty : NodeArray :=
+  .mk #[.false, .false] 1
+
+@[simp, grind =]
+theorem size_empty :
+    empty.size = 1 := by
+  grind [empty]
+
+@[simp, grind =]
+theorem getElem_empty (mem : var ∈ empty) :
+    (empty[var]'mem).toPair = (.false, .false) := by
+  grind [empty]
+
+@[inline]
+instance : Inhabited NodeArray where
+  default := empty
+
+@[always_inline]
+def push (arr : NodeArray) (fst snd : Lit) : NodeArray :=
+  .mk (arr._nodes.push fst |>.push snd) (arr.size + 1)
+
+@[simp, grind =]
+theorem size_push {fst snd : Lit} :
+    (arr.push fst snd).size = arr.size + 1 := by
+  grind [push]
+
+@[simp, grind =]
+theorem getElem_push {fst snd : Lit} (mem : var ∈ (arr.push fst snd)) :
+    ((arr.push fst snd)[var]'mem).toPair =
+    if _ : var ∈ arr then arr[var].toPair else (fst, snd) := by
+  grind [push]
+
+@[always_inline]
+def set (arr : NodeArray) (var : Var) (fst snd : Lit) (mem : var ∈ arr := by get_elem_tactic) : NodeArray :=
+  let baseIdx := 2 * var.idx
+  .mk (arr._nodes.set baseIdx fst |>.set (baseIdx + 1) snd) arr.size
+
+@[simp, grind =]
+theorem size_set (mem : var ∈ arr) {fst snd : Lit} :
+    (arr.set var fst snd mem).size = arr.size := by
+  grind [set]
+
+@[simp, grind =]
+theorem getElem_set {fst snd : Lit} {var' : Var} (mem : var ∈ arr) (mem' : var' ∈ arr.set var fst snd mem) :
+    (arr.set var fst snd mem)[var']'mem' =
+    if var' = var then
+      (fst, snd)
+    else
+      have h : var' ∈ arr := by grind
+      (arr[var']'h).toPair := by
+  grind [set]
+
+end NodeArray
